merged exceptions and function calls

src/imp.v
@@ -8,35 +8,29 @@ Definition F : id := Id 3.
 Definition G : id := Id 4.
 Definition H : id := Id 5.
 
-Definition RET : id := Id 6.
-
+Definition T := ExId 1.
+Definition U := ExId 2.
+Definition V := ExId 3.
 
 Fixpoint aeval (st : state) (a : aexp) : nat :=
   match a with
-  | ANum n => n
-  | AId x => st x
-  | APlus a1 a2 =>
-      (aeval st a1) + (aeval st a2)
-  | AMinus a1 a2  =>
-      (aeval st a1) - (aeval st a2)
-  | AMult a1 a2 =>
-      (aeval st a1) * (aeval st a2)
+    | ANum n        => n
+    | AId x         => st x
+    | APlus a1 a2   => (aeval st a1) + (aeval st a2)
+    | AMinus a1 a2  => (aeval st a1) - (aeval st a2)
+    | AMult a1 a2   => (aeval st a1) * (aeval st a2)
   end.
 
 Fixpoint beval (st : state) (b : bexp) : bool :=
   match b with
-  | BTrue       => true
-  | BFalse      => false
-  | BEq a1 a2   =>
-      beq_nat (aeval st a1) (aeval st a2)
-  | BLe a1 a2   =>
-      ble_nat (aeval  st a1) (aeval st a2)
-  | BNot b1     =>
-      negb (beval st b1)
-  | BAnd b1 b2  =>
-      andb (beval st b1) (beval st b2)
-  end.   
-  
+    | BTrue       => true
+    | BFalse      => false
+    | BEq a1 a2   => beq_nat (aeval st a1) (aeval st a2)
+    | BLe a1 a2   => ble_nat (aeval  st a1) (aeval st a2)
+    | BNot b1     => negb (beval st b1)
+    | BAnd b1 b2  => andb (beval st b1) (beval st b2)
+  end.
+
 Fixpoint zip_state (steval st : state) (ids : list id) (vs : list aexp) : state :=
   match ids with
   | i::ids' => 
@@ -48,7 +42,7 @@ Fixpoint zip_state (steval st : state) (ids : list id) (vs : list aexp) : state 
   	end
   | [] => st
   end.
-
+  
 Fixpoint assigned_vars (c : com) (vars : list id): list id :=
 	match c with
 	| CAss i _ =>
@@ -67,159 +61,80 @@ Inductive ls_disjoint : list id -> list id -> Prop :=
   | LSD_S: forall x xs ys, ls_disjoint xs ys ->
               not (Exists (fun x' => x = x') ys) -> 
               ls_disjoint (x::xs) ys.
-  
-Lemma zip_state_tr : forall steval st st' p q ids r s vs,
-  p <> q ->
-  st = zip_state steval st' (p::q::ids) (r::s::vs) ->
-  st = zip_state steval st' (q::p::ids) (s::r::vs).
-Proof.
-  intros.
-  unfold zip_state. fold zip_state.
-  unfold zip_state in H1. fold zip_state in H1.
-Admitted.
 
-Inductive entry_state : state -> state -> list id -> list aexp -> Prop :=
-  | ES_n: forall steval, entry_state steval empty_state nil nil
-  | ES_S: forall steval st p ps v vs,
-  			entry_state steval st ps vs ->
-  			entry_state steval (update st p (aeval steval v)) (p::ps) (v::vs).
-  
 Inductive list_unique_items {T : Type} : (list T) -> Prop :=
   | LUI_n: list_unique_items []
   | LUI_S: forall xs x, Exists (fun x' => x = x') xs = False -> list_unique_items (x::xs). 
 
-Reserved Notation "c1 ';' program '/' st '||' s '/' st'"
-                  (at level 40, program, st, s at level 39).
-  
-Inductive ceval : com -> program -> state -> status -> state -> Prop :=
-  | E_Skip : forall st program,
-      CSkip ; program / st || SContinue / st
-  | E_Break: forall st program,
-      CBreak ; program / st || SBreak / st
-  | E_Ass : forall st st' ident a n program,
+Reserved Notation "c1 '/' st '||' st'"
+                  (at level 40, st at level 39).
+
+Inductive ceval : com -> program -> state -> state -> option exn -> Prop :=
+  | E_Skip : forall st,
+      CSkip / st || st
+  | E_Ass : forall st st' ident a n,
       aeval st a = n ->
       update st ident n = st' ->
-      CAss ident a ; program / st || SContinue / st'
-  | E_If_True : forall st st' b status c1 c2 program,
+      CAss ident a / st || st'
+  | E_If_True : forall st st' ex b c1 c2 env,
       beval st b = true ->
-      c1 ; program / st || status / st' ->
-      CIf b c1 c2 ; program / st || status / st'
-  | E_If_False : forall st st' b status c1 c2 program,
+      ceval c1 env st st' ex ->
+      ceval (CIf b c1 c2) env st st' ex
+  | E_If_False : forall st st' ex b c1 c2 env,
       beval st b = false ->
-      c2 ; program / st || status / st' ->
-      CIf b c1 c2 ; program / st || status / st'
-  | E_Seq : forall st st' st'' c1 c2 status program,
-      c1 ; program / st || SContinue / st' ->
-      c2 ; program / st' || status / st'' ->
-      CSeq c1 c2 ; program / st || status / st''
-  | E_Seq_Break : forall st st' c1 c2 program,
-      c1 ; program / st || SBreak / st' ->
-      CSeq c1 c2 ; program / st || SBreak / st'
-  | E_While_Break : forall st st' b c program,
-      beval st b = true ->
-      c ; program / st || SBreak / st' ->
-      CWhile b c ; program / st || SContinue / st'
-  | E_While_False : forall st b c program,
+      ceval c2 env st st' ex ->
+      ceval (CIf b c1 c2) env st st' ex
+  | E_Seq : forall st st' st'' c1 c2,
+      c1 / st || st' ->
+      c2 / st' || st'' ->
+      CSeq c1 c2 / st || st''
+  | E_While_False : forall st b c,
       beval st b = false ->
-      CWhile b c ; program / st || SContinue / st
-  | E_While_True : forall st st' st'' b c program,
+      CWhile b c / st || st
+  | E_While_True : forall st st' st'' b c,
       beval st b = true ->
-      c ; program / st || SContinue / st' ->
-      CWhile b c ; program / st' || SContinue / st'' ->
-      CWhile b c ; program / st || SContinue / st''
-  | E_Call : forall st st' st'' entry_st status f program body params args X rexp,
-      program f = (body, params, rexp) ->
+      c / st || st' ->
+      CWhile b c / st' || st'' ->
+      CWhile b c / st || st''
+(* Evidence for throwing and catching exceptions. *)
+  | E_Throw : forall st e aexps ns env,
+      map (fun a => aeval st a) aexps = ns ->
+      ceval (CThrow e aexps) env st st (Some (Exn (e, ns)))
+  | E_Try : forall c1 c2 st st' e ids env,
+      ceval c1 env st st' None ->
+      ceval (CTry c1 e ids c2) env st st' None
+  | E_Catch : forall c1 c2 st st' st'' e ns ids env,
+      ceval c1 env st st' (Some (Exn (e, ns))) ->
+      ceval c2 env (update_many st ids ns) st'' None ->
+      ceval (CTry c1 e ids c2) env st st'' None
+(* Evidence for propagating exceptions out of previously declared constructions. *)
+  | E_Seq1_Exn : forall st st' c1 c2 ex env,
+      ceval c1 env st st' (Some ex) ->
+      ceval (CSeq c1 c2) env st st' (Some ex)
+  | E_Seq2_Exn : forall st st' st'' c1 c2 ex env,
+      c1 / st || st' ->
+      ceval c2 env st' st'' (Some ex) ->
+      ceval (CSeq c1 c2) env st st'' (Some ex)
+  | E_While_Exn : forall st st' b c ex env,
+      beval st b = true ->
+      ceval c env st st' (Some ex) ->
+      ceval (CWhile b c) env st st' (Some ex)
+  | E_Try_Exn : forall c1 c2 st st' e e' ns ids env,
+      e <> e' ->
+      ceval c1 env st st' (Some (Exn (e, ns))) ->
+      ceval (CTry c1 e' ids c2) env st st' (Some (Exn (e, ns)))
+  | E_Catch_Exn : forall c1 c2 st st' st'' e ns ids ex env,
+      ceval c1 env st st' (Some (Exn (e, ns))) ->
+      ceval c2 env (update_many st ids ns) st'' (Some ex) ->
+      ceval (CTry c1 e ids c2) env st st'' (Some ex)
+  | E_Call : forall st st' st'' entry_st f (env : program) body params args X ex rexp,
+      env f = (body, params, rexp) ->
       list_unique_items params ->
       list_unique_items args ->
       length params = length args ->
       ls_disjoint params (assigned_vars body []) ->
       entry_st = zip_state st empty_state params args -> 
-      body ; program / entry_st || status / st'' ->
+      ceval body env entry_st st'' ex ->
       st' = update st X (aeval st'' rexp) ->
-      CCall f X args ; program / st || SContinue / st'
-     
-  (* | E_Call : forall st st' st'' entry_st status f program body params args X rexp,
-      program f = (body, params, rexp) ->
-      entry_st = update empty_state params (aeval st args) -> 
-      body ; program / entry_st || status / st'' ->
-      st' = update st X (aeval st'' rexp) ->
-      CCall f X args ; program / st || SContinue / st' *)
-      
-  (*| E_Call : forall st st' status f program body params args X rexp,
-      program f = (body, params, rexp) ->
-      body ; program / st || status / st' ->
-      CCall f X args ; program / st || SContinue / st' *)
-      
-  (*| E_Call : forall st st' st'' ident status p program c rexp params args entry_st x,
-      program p = (c, params, rexp) ->
-      length params = length args ->
-      entry_st = update st params args ->
-      c / entry_st || status / st ->
-      x = aeval st rexp ->
-      st'' = update st' ident x ->
-      CCall ident p args / st' || SContinue / st'' *)
-
-  where "c1 ';' program '/' st '||' s '/' st'" := (ceval c1 program st s st').
-  
-(*Theorem ceval_deterministic: forall (c:com) st st1 st2 s1 s2,
-     c / st || s1 / st1  ->
-     c / st || s2 / st2 ->
-     st1 = st2 /\ s1 = s2.
-Proof.
-  intros.
-  generalize dependent s2.
-  generalize dependent st2.
-  induction H0; intros.
-  Case "E_Skip". inversion H1; subst; split; reflexivity.
-  Case "E_Break". inversion H1; subst; split; reflexivity.
-  Case "E_Ass". inversion H2; subst; split; reflexivity.
-  Case "E_If_True".
-    inversion H2; subst.
-    apply IHceval', H10.
-    rewrite H0 in H9; inversion H9.
-  Case "E_If_False".
-    inversion H2; subst.
-    rewrite H0 in H9; inversion H9.
-    apply IHceval'; apply H10.
-  Case "E_Seq".
-    inversion H1; subst.
-    specialize (IHceval'1 _ _ H3).
-    destruct IHceval'1; subst.    
-    apply IHceval'2, H7.
-    specialize (IHceval'1 _ _ H6).
-    destruct IHceval'1.
-    congruence.
-  Case "E_Seq_Break".
-    inversion H1; subst.
-    specialize (IHceval' _ _ H4); subst.
-    destruct IHceval'.
-    congruence.
-    apply IHceval'.
-    assumption.
-  Case "E_While_Break".
-    inversion H2; subst.
-    specialize (IHceval' _ _ H9).
-    destruct IHceval'.
-    split; [ assumption | reflexivity ].
-    congruence.
-    specialize (IHceval' _ _ H6).
-    destruct IHceval'.
-    congruence.
-  Case "E_While_False".
-    inversion H1; subst.
-    congruence.
-    split; reflexivity.
-    congruence.
-  Case "E_While_True".
-    inversion H1; subst.
-    specialize (IHceval'1 _ _ H8).
-    destruct IHceval'1.
-    congruence.
-    congruence.
-    specialize (IHceval'1 _ _ H5); destruct IHceval'1; subst.
-    specialize (IHceval'2 _ _ H9); assumption. 
-  Case "E_Call".
-    inversion H6; subst.
-    specialize (IHceval' _ _ H3).
-    subst.
-Qed.*)
+      ceval (CCall f X args) env st st' ex
+  where "c1 '/' st '||' st'" := (forall env, (ceval c1 env st st' None)).
