src/imp_ast.v
@@ -3,7 +3,13 @@ Require Import Coq.Arith.Peano_dec.
 
 Inductive id : Type :=
   | Id : nat -> id.
-  
+
+Inductive exid : Type :=
+  | ExId : nat -> exid.
+
+Inductive exn : Type :=
+  | Exn : exid * list nat -> exn.
+
 Theorem eq_id_dec : forall id1 id2 : id, {id1 = id2} + {id1 <> id2}.
 Proof.
    intros id1 id2.
@@ -13,7 +19,18 @@ Proof.
      left. rewrite Heq. reflexivity.
    Case "n1 <> n2".
      right. intros contra. inversion contra. apply Hneq. apply H0.
-Defined. 
+Defined.
+
+Theorem eq_exid_dec : forall e1 e2 : exid, {e1 = e2} + {e1 <> e2}.
+Proof.
+   intros e1 e2.
+   destruct e1 as [n1]. destruct e2 as [n2].
+   destruct (eq_nat_dec n1 n2) as [Heq | Hneq].
+   Case "n1 = n2".
+     left. rewrite Heq. reflexivity.
+   Case "n1 <> n2".
+     right. intros contra. inversion contra. apply Hneq. apply H0.
+Defined.
 
 Inductive aexp : Type :=
   | ANum : nat -> aexp
@@ -21,7 +38,7 @@ Inductive aexp : Type :=
   | APlus : aexp -> aexp -> aexp
   | AMinus : aexp -> aexp -> aexp
   | AMult : aexp -> aexp -> aexp.
-  
+
 Inductive bexp : Type :=
   | BTrue : bexp
   | BFalse : bexp
@@ -29,16 +46,17 @@ Inductive bexp : Type :=
   | BLe : aexp -> aexp -> bexp
   | BNot : bexp -> bexp
   | BAnd : bexp -> bexp -> bexp.
-  
+
 Inductive com : Type :=
   | CSkip : com
-  | CBreak : com
   | CAss : id -> aexp -> com
   | CSeq : com -> com -> com
   | CIf : bexp -> com -> com -> com
   | CWhile : bexp -> com -> com
+  | CThrow : exid -> list aexp -> com
+  | CTry : com -> exid -> list id -> com -> com
   | CCall : id -> id -> list aexp -> com.
-  
+
 Notation "'SKIP'" :=
   CSkip.
 Notation "X '::=' a" :=
@@ -49,3 +67,7 @@ Notation "'IFB' e1 'THEN' e2 'ELSE' e3 'FI'" :=
   (CIf e1 e2 e3) (at level 80, right associativity).
 Notation "'WHILE' b 'DO' c 'END'" :=
   (CWhile b c) (at level 80, right associativity).
+Notation "'THROW' ex ',' aexps" :=
+  (CThrow ex aexps) (at level 60).
+Notation "'TRY' c1 'CATCH' ex ',' ids 'DO' c2 'END'" :=
+  (CTry c1 ex ids c2) (at level 80, right associativity).
